store/client_proofs/connect.v
@@ -47,10 +47,10 @@ iIntros "!> %Φ client post".
 rewrite /Client.connect.
 wp_pure _ credit:"c1". wp_pure _ credit:"c2". wp_pures.
 wp_apply (wp_connection_connect with "[//] [//] [//] [] []") => //.
-iIntros "%cs (#sess & ts & % & % & %e_rl & token)".
+iIntros "%cs (#sess & ts & % & % & %e_rl & rel & token)".
 iDestruct "client" as "(%beginning & client)".
 iMod (client_connectingI with "[//] [$] sess token client")
-  as "{sess} (client & #conn & rel & #ready)" => //; try solve_ndisj.
+  as "{sess} (client & #conn & #ready)" => //; try solve_ndisj.
 subst kI kR.
 iPoseProof (init_predI _ _ (TInt 0) with "client []") as "#?".
 { iApply (session_failed_for_orE with "ready").
